obligations tableaux: refonte totale; log pour why-viewer
git-svn-id: https://www.lri.fr/svn/demons/why2/trunk@385 ecafba89-7d34-45a1-8a0b-92829e960b72

bench/good-c/all.c
@@ -23,9 +23,8 @@ int t[];
 
 void t1() /*@ array_length(t) = 10 and t[0] = 1 */ { y = t[0]; } /*@ y = 1 */
 
-/* BUG CALCUL WP */
-/* void t2() */
-/* @ array_length(t) = 10 and x = 0 and t[0] = 1 * / { y = t[x++]; } /*@ y = 1 */
+void t2()
+/*@ array_length(t) = 10 and x = 0 and t[0] = 1 */ { y = t[x++]; } /*@ y = 1 */
 
 /* void t3() */
 /* @ array_length(t) = 10 and x = 0 and t[1] = 1 * / { y = t[++x]; } /*@ y = 1 */
