src/log.mli
@@ -1,0 +1,7 @@
+
+(* Exported type for the why-viewer:
+   (position, predicate, is automatically dicharged)
+*)
+
+type t = (int * string * bool) list
+
