bench/good-c/all_why.v
@@ -185,16 +185,70 @@ Definition t1 := (* validation *)
       (t1_po_2 t Pre2 Pre1)) in
     (exist_2 [y1: Z][result0: unit]`y1 = 1` result tt Post1).
 
+Lemma t2_po_1 : 
+  (t: (array Z))
+  (x: Z)
+  (Pre2: `(array_length t) = 10` /\ `x = 0` /\ `(access t 0) = 1`)
+  (c_aux_2: Z)
+  (Post2: c_aux_2 = x)
+  (x0: Z)
+  (Post1: x0 = `x + 1`)
+  `(access t c_aux_2) = 1` /\ `0 <= c_aux_2` /\ `c_aux_2 < (array_length t)`.
+Proof.
+Intuition.
+Subst c_aux_2 x; Auto.
+Save.
+
+Lemma t2_po_2 : 
+  (t: (array Z))
+  (x: Z)
+  (Pre2: `(array_length t) = 10` /\ `x = 0` /\ `(access t 0) = 1`)
+  (aux_1: Z)
+  (Post4: `(access t aux_1) = 1` /\ `0 <= aux_1` /\
+          `aux_1 < (array_length t)`)
+  `0 <= aux_1` /\ `aux_1 < (array_length t)`.
+Proof.
+Intuition.
+Save.
+
+Definition t2 := (* validation *)
+  [_: unit; t: (array Z); x: Z; y: Z; Pre2: `(array_length t) = 10` /\
+   `x = 0` /\ `(access t 0) = 1`]
+    let (x0, result, Post3) =
+      let (x0, aux_1, Post4) =
+        let (c_aux_2, Post2) = (exist_1 [result: Z]result = x x
+          (refl_equal ? x)) in
+        let (x0, result, Post5) =
+          let (x0, result, Post1) =
+            let (result, Post1) = (exist_1 [result: Z]
+              result = `x + 1` `x + 1` (refl_equal ? `x + 1`)) in
+            (exist_2 [x1: Z][result0: unit]x1 = `x + 1` result tt Post1) in
+          let (result0, Post6) = (exist_1 [result0: Z]
+            `(access t result0) = 1` /\ `0 <= result0` /\
+            `result0 < (array_length t)` c_aux_2
+            (t2_po_1 t x Pre2 c_aux_2 Post2 x0 Post1)) in
+          (exist_2 [x1: Z][result1: Z]`(access t result1) = 1` /\
+          `0 <= result1` /\ `result1 < (array_length t)` x0 result0 Post6) in
+        (exist_2 [x1: Z][result0: Z]`(access t result0) = 1` /\
+        `0 <= result0` /\ `result0 < (array_length t)` x0 result Post5) in
+      let Pre1 = (t2_po_2 t x Pre2 aux_1 Post4) in
+      let (result, Post7) =
+        let (result, Post8) = (exist_1 [result: Z]
+          `(access t result) = 1` aux_1 (proj1 ? ? Post4)) in
+        (exist_1 [result0: Z]`result0 = 1` (access t result) Post8) in
+      (exist_2 [x1: Z][result0: Z]`result0 = 1` x0 result Post7) in
+    (exist_3 [x1: Z][y1: Z][result0: unit]`y1 = 1` x0 result tt Post3).
+
 Lemma e1_po_1 : 
   (x: Z)
   (Pre1: `x = 2`)
-  (c_aux_2: Z)
-  (Post3: c_aux_2 = x)
   (c_aux_3: Z)
-  (Post2: c_aux_3 = x)
+  (Post3: c_aux_3 = x)
+  (c_aux_4: Z)
+  (Post2: c_aux_4 = x)
   (x0: Z)
   (Post1: x0 = `x + 1`)
-  `c_aux_2 + c_aux_3 = 4`.
+  `c_aux_3 + c_aux_4 = 4`.
 Proof.
 Intuition.
 Save.
@@ -202,11 +256,11 @@ Save.
 Definition e1 := (* validation *)
   [_: unit; x: Z; y: Z; Pre1: `x = 2`]
     let (x0, result, Post4) =
-      let (c_aux_2, Post3) = (exist_1 [result: Z]result = x x
+      let (c_aux_3, Post3) = (exist_1 [result: Z]result = x x
         (refl_equal ? x)) in
       let (x0, result, Post5) =
-        let (x0, c_aux_4, Post6) =
-          let (c_aux_3, Post2) = (exist_1 [result: Z]result = x x
+        let (x0, c_aux_5, Post6) =
+          let (c_aux_4, Post2) = (exist_1 [result: Z]result = x x
             (refl_equal ? x)) in
           let (x0, result, Post7) =
             let (x0, result, Post1) =
@@ -214,14 +268,14 @@ Definition e1 := (* validation *)
                 result = `x + 1` `x + 1` (refl_equal ? `x + 1`)) in
               (exist_2 [x1: Z][result0: unit]x1 = `x + 1` result tt Post1) in
             let (result0, Post8) = (exist_1 [result0: Z]
-              `c_aux_2 + result0 = 4` c_aux_3
-              (e1_po_1 x Pre1 c_aux_2 Post3 c_aux_3 Post2 x0 Post1)) in
-            (exist_2 [x1: Z][result1: Z]`c_aux_2 + result1 = 4` x0 result0
+              `c_aux_3 + result0 = 4` c_aux_4
+              (e1_po_1 x Pre1 c_aux_3 Post3 c_aux_4 Post2 x0 Post1)) in
+            (exist_2 [x1: Z][result1: Z]`c_aux_3 + result1 = 4` x0 result0
             Post8) in
-          (exist_2 [x1: Z][result0: Z]`c_aux_2 + result0 = 4` x0 result
+          (exist_2 [x1: Z][result0: Z]`c_aux_3 + result0 = 4` x0 result
           Post7) in
         let (result, Post9) = (exist_1 [result: Z]
-          `result = 4` `c_aux_2 + c_aux_4` Post6) in
+          `result = 4` `c_aux_3 + c_aux_5` Post6) in
         (exist_2 [x1: Z][result0: Z]`result0 = 4` x0 result Post9) in
       (exist_2 [x1: Z][result0: Z]`result0 = 4` x0 result Post5) in
     (exist_3 [x1: Z][y1: Z][result0: unit]`y1 = 4` x0 result tt Post4).
@@ -229,11 +283,11 @@ Definition e1 := (* validation *)
 Lemma e2_po_1 : 
   (x: Z)
   (Pre1: `x = 2`)
-  (c_aux_5: Z)
-  (Post2: c_aux_5 = x)
+  (c_aux_6: Z)
+  (Post2: c_aux_6 = x)
   (x0: Z)
   (Post1: x0 = `x + 1`)
-  `c_aux_5 + x0 = 5`.
+  `c_aux_6 + x0 = 5`.
 Proof.
 Intuition.
 Save.
@@ -241,21 +295,21 @@ Save.
 Definition e2 := (* validation *)
   [_: unit; x: Z; y: Z; Pre1: `x = 2`]
     let (x0, result, Post3) =
-      let (c_aux_5, Post2) = (exist_1 [result: Z]result = x x
+      let (c_aux_6, Post2) = (exist_1 [result: Z]result = x x
         (refl_equal ? x)) in
       let (x0, result, Post4) =
-        let (x0, c_aux_6, Post5) =
+        let (x0, c_aux_7, Post5) =
           let (x0, result, Post1) =
             let (result, Post1) = (exist_1 [result: Z]
               result = `x + 1` `x + 1` (refl_equal ? `x + 1`)) in
             (exist_2 [x1: Z][result0: unit]x1 = `x + 1` result tt Post1) in
           let (result0, Post6) = (exist_1 [result0: Z]
-            `c_aux_5 + result0 = 5` x0
-            (e2_po_1 x Pre1 c_aux_5 Post2 x0 Post1)) in
-          (exist_2 [x1: Z][result1: Z]`c_aux_5 + result1 = 5` x0 result0
+            `c_aux_6 + result0 = 5` x0
+            (e2_po_1 x Pre1 c_aux_6 Post2 x0 Post1)) in
+          (exist_2 [x1: Z][result1: Z]`c_aux_6 + result1 = 5` x0 result0
           Post6) in
         let (result, Post7) = (exist_1 [result: Z]
-          `result = 5` `c_aux_5 + c_aux_6` Post5) in
+          `result = 5` `c_aux_6 + c_aux_7` Post5) in
         (exist_2 [x1: Z][result0: Z]`result0 = 5` x0 result Post7) in
       (exist_2 [x1: Z][result0: Z]`result0 = 5` x0 result Post4) in
     (exist_3 [x1: Z][y1: Z][result0: unit]`y1 = 5` x0 result tt Post3).
@@ -263,11 +317,11 @@ Definition e2 := (* validation *)
 Lemma e3_po_1 : 
   (x: Z)
   (Pre1: `x = 2`)
-  (c_aux_7: Z)
-  (Post2: c_aux_7 = x)
+  (c_aux_8: Z)
+  (Post2: c_aux_8 = x)
   (x0: Z)
   (Post1: x0 = `x + 1`)
-  ((result:Z) (result = x0 -> `c_aux_7 + result = 5`)).
+  ((result:Z) (result = x0 -> `c_aux_8 + result = 5`)).
 Proof.
 Intuition.
 Save.
@@ -276,11 +330,11 @@ Lemma e3_po_2 :
   (x: Z)
   (Pre1: `x = 2`)
   (x0: Z)
-  (c_aux_8: Z)
-  (Post5: ((result:Z) (result = x0 -> `c_aux_8 + result = 5`)))
   (c_aux_9: Z)
-  (Post3: c_aux_9 = x0)
-  `c_aux_8 + c_aux_9 = 5`.
+  (Post5: ((result:Z) (result = x0 -> `c_aux_9 + result = 5`)))
+  (c_aux_10: Z)
+  (Post3: c_aux_10 = x0)
+  `c_aux_9 + c_aux_10 = 5`.
 Proof.
 Intuition.
 Save.
@@ -288,8 +342,8 @@ Save.
 Definition e3 := (* validation *)
   [_: unit; x: Z; y: Z; Pre1: `x = 2`]
     let (x0, result, Post4) =
-      let (x0, c_aux_8, Post5) =
-        let (c_aux_7, Post2) = (exist_1 [result: Z]result = x x
+      let (x0, c_aux_9, Post5) =
+        let (c_aux_8, Post2) = (exist_1 [result: Z]result = x x
           (refl_equal ? x)) in
         let (x0, result, Post6) =
           let (x0, result, Post1) =
@@ -297,19 +351,19 @@ Definition e3 := (* validation *)
               result = `x + 1` `x + 1` (refl_equal ? `x + 1`)) in
             (exist_2 [x1: Z][result0: unit]x1 = `x + 1` result tt Post1) in
           let (result0, Post7) = (exist_1 [result0: Z]
-            ((result:Z) (result = x0 -> `result0 + result = 5`)) c_aux_7
-            (e3_po_1 x Pre1 c_aux_7 Post2 x0 Post1)) in
+            ((result:Z) (result = x0 -> `result0 + result = 5`)) c_aux_8
+            (e3_po_1 x Pre1 c_aux_8 Post2 x0 Post1)) in
           (exist_2 [x1: Z][result1: Z]
           ((result:Z) (result = x1 -> `result1 + result = 5`)) x0 result0
           Post7) in
         (exist_2 [x1: Z][result0: Z]
         ((result:Z) (result = x1 -> `result0 + result = 5`)) x0 result Post6) in
       let (result, Post8) =
-        let (c_aux_9, Post3) = (exist_1 [result: Z]result = x0 x0
+        let (c_aux_10, Post3) = (exist_1 [result: Z]result = x0 x0
           (refl_equal ? x0)) in
         let (result, Post9) = (exist_1 [result: Z]
-          `result = 5` `c_aux_8 + c_aux_9`
-          (e3_po_2 x Pre1 x0 c_aux_8 Post5 c_aux_9 Post3)) in
+          `result = 5` `c_aux_9 + c_aux_10`
+          (e3_po_2 x Pre1 x0 c_aux_9 Post5 c_aux_10 Post3)) in
         (exist_1 [result0: Z]`result0 = 5` result Post9) in
       (exist_2 [x1: Z][result0: Z]`result0 = 5` x0 result Post8) in
     (exist_3 [x1: Z][y1: Z][result0: unit]`y1 = 5` x0 result tt Post4).
@@ -328,11 +382,11 @@ Lemma e4_po_2 :
   (x: Z)
   (Pre1: `x = 2`)
   (x0: Z)
-  (c_aux_10: Z)
-  (Post4: ((result:Z) (result = x0 -> `c_aux_10 + result = 6`)))
   (c_aux_11: Z)
-  (Post2: c_aux_11 = x0)
-  `c_aux_10 + c_aux_11 = 6`.
+  (Post4: ((result:Z) (result = x0 -> `c_aux_11 + result = 6`)))
+  (c_aux_12: Z)
+  (Post2: c_aux_12 = x0)
+  `c_aux_11 + c_aux_12 = 6`.
 Proof.
 Intuition.
 Save.
@@ -340,7 +394,7 @@ Save.
 Definition e4 := (* validation *)
   [_: unit; x: Z; y: Z; Pre1: `x = 2`]
     let (x0, result, Post3) =
-      let (x0, c_aux_10, Post4) =
+      let (x0, c_aux_11, Post4) =
         let (x0, result, Post1) =
           let (result, Post1) = (exist_1 [result: Z]result = `x + 1` 
             `x + 1` (refl_equal ? `x + 1`)) in
@@ -352,11 +406,11 @@ Definition e4 := (* validation *)
         ((result:Z) (result = x1 -> `result1 + result = 6`)) x0 result0
         Post5) in
       let (result, Post6) =
-        let (c_aux_11, Post2) = (exist_1 [result: Z]result = x0 x0
+        let (c_aux_12, Post2) = (exist_1 [result: Z]result = x0 x0
           (refl_equal ? x0)) in
         let (result, Post7) = (exist_1 [result: Z]
-          `result = 6` `c_aux_10 + c_aux_11`
-          (e4_po_2 x Pre1 x0 c_aux_10 Post4 c_aux_11 Post2)) in
+          `result = 6` `c_aux_11 + c_aux_12`
+          (e4_po_2 x Pre1 x0 c_aux_11 Post4 c_aux_12 Post2)) in
         (exist_1 [result0: Z]`result0 = 6` result Post7) in
       (exist_2 [x1: Z][result0: Z]`result0 = 6` x0 result Post6) in
     (exist_3 [x1: Z][y1: Z][result0: unit]`y1 = 6` x0 result tt Post3).
@@ -375,14 +429,14 @@ Lemma e5_po_2 :
   (x: Z)
   (Pre1: `x = 2`)
   (x0: Z)
-  (c_aux_12: Z)
-  (Post5: ((result:Z)
-           (result = x0 -> ((x:Z) (x = `x0 + 1` -> `c_aux_12 + result = 6`)))))
   (c_aux_13: Z)
-  (Post3: c_aux_13 = x0)
+  (Post5: ((result:Z)
+           (result = x0 -> ((x:Z) (x = `x0 + 1` -> `c_aux_13 + result = 6`)))))
+  (c_aux_14: Z)
+  (Post3: c_aux_14 = x0)
   (x1: Z)
   (Post2: x1 = `x0 + 1`)
-  `c_aux_12 + c_aux_13 = 6`.
+  `c_aux_13 + c_aux_14 = 6`.
 Proof.
 Intuition.
 Save.
@@ -390,7 +444,7 @@ Save.
 Definition e5 := (* validation *)
   [_: unit; x: Z; y: Z; Pre1: `x = 2`]
     let (x0, result, Post4) =
-      let (x0, c_aux_12, Post5) =
+      let (x0, c_aux_13, Post5) =
         let (x0, result, Post1) =
           let (result, Post1) = (exist_1 [result: Z]result = `x + 1` 
             `x + 1` (refl_equal ? `x + 1`)) in
@@ -404,8 +458,8 @@ Definition e5 := (* validation *)
          (result = x1 -> ((x:Z) (x = `x1 + 1` -> `result1 + result = 6`)))) 
         x0 result0 Post6) in
       let (x1, result, Post7) =
-        let (x1, c_aux_14, Post8) =
-          let (c_aux_13, Post3) = (exist_1 [result: Z]result = x0 x0
+        let (x1, c_aux_15, Post8) =
+          let (c_aux_14, Post3) = (exist_1 [result: Z]result = x0 x0
             (refl_equal ? x0)) in
           let (x1, result, Post9) =
             let (x1, result, Post2) =
@@ -413,14 +467,14 @@ Definition e5 := (* validation *)
                 result = `x0 + 1` `x0 + 1` (refl_equal ? `x0 + 1`)) in
               (exist_2 [x2: Z][result0: unit]x2 = `x0 + 1` result tt Post2) in
             let (result0, Post10) = (exist_1 [result0: Z]
-              `c_aux_12 + result0 = 6` c_aux_13
-              (e5_po_2 x Pre1 x0 c_aux_12 Post5 c_aux_13 Post3 x1 Post2)) in
-            (exist_2 [x2: Z][result1: Z]`c_aux_12 + result1 = 6` x1 result0
+              `c_aux_13 + result0 = 6` c_aux_14
+              (e5_po_2 x Pre1 x0 c_aux_13 Post5 c_aux_14 Post3 x1 Post2)) in
+            (exist_2 [x2: Z][result1: Z]`c_aux_13 + result1 = 6` x1 result0
             Post10) in
-          (exist_2 [x2: Z][result0: Z]`c_aux_12 + result0 = 6` x1 result
+          (exist_2 [x2: Z][result0: Z]`c_aux_13 + result0 = 6` x1 result
           Post9) in
         let (result, Post11) = (exist_1 [result: Z]
-          `result = 6` `c_aux_12 + c_aux_14` Post8) in
+          `result = 6` `c_aux_13 + c_aux_15` Post8) in
         (exist_2 [x2: Z][result0: Z]`result0 = 6` x1 result Post11) in
       (exist_2 [x2: Z][result0: Z]`result0 = 6` x1 result Post7) in
     (exist_3 [x1: Z][y1: Z][result0: unit]`y1 = 6` x0 result tt Post4).
