examples/heapsort/swap_why.v
@@ -13,6 +13,7 @@ Lemma swap_po_1 :
   (Pre4: `0 <= i` /\ `i < (array_length t)`)
   (v: Z)
   (Post3: v = (access t i))
+  (Pre2: `0 <= i` /\ `i < (array_length t)`)
   `0 <= j` /\ `j < (array_length t)`.
 Proof.
 Intros; Omega.
@@ -27,12 +28,13 @@ Lemma swap_po_2 :
   (Pre4: `0 <= i` /\ `i < (array_length t)`)
   (v: Z)
   (Post3: v = (access t i))
+  (Pre2: `0 <= i` /\ `i < (array_length t)`)
   (Pre3: `0 <= j` /\ `j < (array_length t)`)
-  (result: Z)
-  (Post1: (store t i result) = (store t i (access t j)))
-  `0 <= i` /\ `i < (array_length (store t i result))`.
+  (t0: (array Z))
+  (Post1: t0 = (store t i (access t j)))
+  `0 <= j` /\ `j < (array_length t0)`.
 Proof.
-Intros; Simpl; Omega.
+Intros; ArraySubst t0.
 Save.
 
 Lemma swap_po_3 : 
@@ -44,28 +46,11 @@ Lemma swap_po_3 :
   (Pre4: `0 <= i` /\ `i < (array_length t)`)
   (v: Z)
   (Post3: v = (access t i))
+  (Pre2: `0 <= i` /\ `i < (array_length t)`)
   (Pre3: `0 <= j` /\ `j < (array_length t)`)
   (t0: (array Z))
   (Post1: t0 = (store t i (access t j)))
-  (result0: Z)
-  (Post2: (store t0 j result0) = (store t0 j v))
-  `0 <= j` /\ `j < (array_length (store t0 j result0))`.
-Proof.
-Intros; ArraySubst t0.
-Save.
-
-Lemma swap_po_4 : 
-  (i: Z)
-  (j: Z)
-  (t: (array Z))
-  (Pre5: (`0 <= i` /\ `i < (array_length t)`) /\ `0 <= j` /\
-         `j < (array_length t)`)
-  (Pre4: `0 <= i` /\ `i < (array_length t)`)
-  (v: Z)
-  (Post3: v = (access t i))
-  (Pre3: `0 <= j` /\ `j < (array_length t)`)
-  (t0: (array Z))
-  (Post1: t0 = (store t i (access t j)))
+  (Pre1: `0 <= j` /\ `j < (array_length t0)`)
   (t1: (array Z))
   (Post2: t1 = (store t0 j v))
   (exchange t1 t i j).
@@ -81,24 +66,17 @@ Definition swap := (* validation *)
     let (v, Post3) = (exist_1 [result: Z]result = (access t i) (access t i)
       (refl_equal ? (access t i))) in
     let (t0, result, Post4) =
-      let Pre3 = (swap_po_1 i j t Pre5 Pre4 v Post3) in
-      let (t0, result, Post1) =
-        let (result, Post1) = (exist_1 [result: Z]
-          (store t i result) = (store t i (access t j)) (access t j)
-          (refl_equal ? (store t i (access t j)))) in
-        let Pre1 = (swap_po_2 i j t Pre5 Pre4 v Post3 Pre3 result Post1) in
-        (exist_2 [t1: (array Z)][result1: unit]
-        t1 = (store t i (access t j)) (store t i result) tt Post1) in
-      let (t1, result0, Post2) =
-        let (result0, Post2) = (exist_1 [result0: Z]
-          (store t0 j result0) = (store t0 j v) v
-          (refl_equal ? (store t0 j v))) in
-        let Pre2 =
-          (swap_po_3 i j t Pre5 Pre4 v Post3 Pre3 t0 Post1 result0 Post2) in
-        (exist_2 [t2: (array Z)][result2: unit]
-        t2 = (store t0 j v) (store t0 j result0) tt Post2) in
+      let Pre2 = Pre4 in
+      let Pre3 = (swap_po_1 i j t Pre5 Pre4 v Post3 Pre2) in
+      let (t0, result, Post1) = (exist_2 [t1: (array Z)][result1: unit]
+        t1 = (store t i (access t j)) (store t i (access t j)) tt
+        (refl_equal ? (store t i (access t j)))) in
+      let Pre1 = (swap_po_2 i j t Pre5 Pre4 v Post3 Pre2 Pre3 t0 Post1) in
+      let (t1, result0, Post2) = (exist_2 [t2: (array Z)][result2: unit]
+        t2 = (store t0 j v) (store t0 j v) tt
+        (refl_equal ? (store t0 j v))) in
       (exist_2 [t2: (array Z)][result1: unit](exchange t2 t i j) t1 result0
-      (swap_po_4 i j t Pre5 Pre4 v Post3 Pre3 t0 Post1 t1 Post2)) in
+      (swap_po_3 i j t Pre5 Pre4 v Post3 Pre2 Pre3 t0 Post1 Pre1 t1 Post2)) in
     (exist_2 [t1: (array Z)][result0: unit](exchange t1 t i j) t0 result
     Post4).
 
